code/experimental/P256/Hacl.Impl.ECDSA.P256SHA256.Signature.fst
@@ -30,16 +30,52 @@ open FStar.Mul
 
 #set-options "--z3rlimit 100"
 
+val lemma_core_0: a: lbuffer uint64 (size 4) -> h: mem -> 
+  Lemma (Lib.ByteSequence.nat_from_intseq_le (as_seq h a) == as_nat h a)
+
+let lemma_core_0 a h = 
+  let open Lib.ByteSequence in 
+  
+    let k = as_seq h a in 
+    let z = nat_from_intseq_le k in 
+    
+    nat_from_intseq_le_slice_lemma k 1;
+    nat_from_intseq_le_lemma0 (Seq.slice k 0 1);
+
+    let k1 = Seq.slice k 1 4 in 
+      nat_from_intseq_le_slice_lemma #_ #_ #3 k1 1;
+      nat_from_intseq_le_lemma0 (Seq.slice k1 0 1);
+      
+    let k2 = Seq.slice k1 1 3 in 
+      nat_from_intseq_le_slice_lemma #_ #_ #2 k2 1;
+      nat_from_intseq_le_lemma0 (Seq.slice k2 0 1);
+      nat_from_intseq_le_lemma0 (Seq.slice k2 1 2)
+
+
+val lemma_core_1: a: lbuffer uint64 (size 4) -> h: mem -> 
+  Lemma (Lib.ByteSequence.nat_from_bytes_le (Lib.ByteSequence.uints_to_bytes_le (as_seq h a)) == as_nat h a)
+
+let lemma_core_1 a h= 
+  let open Lib.ByteSequence in 
+  let k = as_seq h a in 
+  let z = Lib.ByteSequence.uints_to_bytes_le (as_seq h a) in 
+  let maint = Lib.ByteSequence.nat_from_bytes_le (Lib.ByteSequence.uints_to_bytes_le (as_seq h a)) in 
+  lemma_core_0 a h;
+  lemma_nat_from_to_intseq_le_preserves_value #U64 #SEC 4 (as_seq h a);
+  let n = nat_from_intseq_le k in 
+  uints_to_bytes_le_nat_lemma #U64 #SEC 4 n;
+  lemma_nat_to_from_bytes_le_preserves_value #SEC (uints_to_bytes_le #U64 #SEC #4 (as_seq h a)) 32 (as_nat h a)
+
 
 val ecdsa_signature_step12: mLen: size_t -> m: lbuffer uint8 mLen {uint_v mLen < pow2 61} -> hashAsFelem: felem -> 
   Stack unit 
     (requires fun h -> live h m /\ live h hashAsFelem)
     (ensures fun h0 _ h1 -> modifies (loc hashAsFelem) h0 h1 /\
       (
-	let hashOfMessage = Spec.Hash.hash Spec.Hash.Definitions.SHA2_256 (as_seq h0 m) in 
-	let changedEndianHash = Hacl.Spec.ECDSA.changeEndian (Lib.ByteSequence.uints_from_bytes_be hashOfMessage) in 
-	as_nat h1 hashAsFelem == felem_seq_as_nat changedEndianHash % prime_p256_order 
-      )
+	let hashM = Spec.Hash.hash Spec.Hash.Definitions.SHA2_256 (as_seq h0 m) in 
+	let hashChanged = Hacl.Spec.ECDSA.changeEndian (Lib.ByteSequence.uints_from_bytes_be hashM) in 
+	as_nat h1 hashAsFelem == (Lib.ByteSequence.nat_from_intseq_le hashChanged) % prime_p256_order
+      ) 
   ) 
 
 let ecdsa_signature_step12 mLen m hashAsFelem  = 
@@ -49,8 +85,7 @@ let ecdsa_signature_step12 mLen m hashAsFelem  =
     hash_256 m mLen mHash;
     toUint64ChangeEndian mHash hashAsFelem;
       let h2 = ST.get() in 
-      lemma_eq_funct (as_seq h2 hashAsFelem) (Hacl.Spec.ECDSA.changeEndian 
-	(Lib.ByteSequence.uints_from_bytes_be (Spec.Hash.hash Spec.Hash.Definitions.SHA2_256 (as_seq h0 m))));
+      lemma_core_0 hashAsFelem h2;
     reduction_prime_2prime_order hashAsFelem hashAsFelem;
   pop_frame()
 
@@ -173,47 +208,9 @@ let toUint64 i o =
 
 
 
-val lemma_core_0: a: lbuffer uint64 (size 4) -> h: mem -> 
-  Lemma (Lib.ByteSequence.nat_from_intseq_le (as_seq h a) == as_nat h a)
-
-let lemma_core_0 a h = 
-  let open Lib.ByteSequence in 
-  
-    let k = as_seq h a in 
-    let z = nat_from_intseq_le k in 
-    
-    nat_from_intseq_le_slice_lemma k 1;
-    nat_from_intseq_le_lemma0 (Seq.slice k 0 1);
-
-    let k1 = Seq.slice k 1 4 in 
-      nat_from_intseq_le_slice_lemma #_ #_ #3 k1 1;
-      nat_from_intseq_le_lemma0 (Seq.slice k1 0 1);
-      
-    let k2 = Seq.slice k1 1 3 in 
-      nat_from_intseq_le_slice_lemma #_ #_ #2 k2 1;
-      nat_from_intseq_le_lemma0 (Seq.slice k2 0 1);
-      nat_from_intseq_le_lemma0 (Seq.slice k2 1 2)
-
-
-val lemma_core_1: a: lbuffer uint64 (size 4) -> h: mem -> 
-  Lemma (Lib.ByteSequence.nat_from_bytes_le (Lib.ByteSequence.uints_to_bytes_le (as_seq h a)) == as_nat h a)
-
-let lemma_core_1 a h= 
-  let open Lib.ByteSequence in 
-  let k = as_seq h a in 
-  let z = Lib.ByteSequence.uints_to_bytes_le (as_seq h a) in 
-  let maint = Lib.ByteSequence.nat_from_bytes_le (Lib.ByteSequence.uints_to_bytes_le (as_seq h a)) in 
-  lemma_core_0 a h;
-  lemma_nat_from_to_intseq_le_preserves_value #U64 #SEC 4 (as_seq h a);
-  let n = nat_from_intseq_le k in 
-  uints_to_bytes_le_nat_lemma #U64 #SEC 4 n;
-  lemma_nat_to_from_bytes_le_preserves_value #SEC (uints_to_bytes_le #U64 #SEC #4 (as_seq h a)) 32 (as_nat h a)
-
-
-
 
 val ecdsa_signature_core_nist_compliant: m: lbuffer uint8 (size 32) -> 
-  privKeyAsFelem: felem  -> 
+  privKeyAsFelem: felem -> 
   k: lbuffer uint8 (size 32) -> 
   r: felem -> 
   s: felem -> 
@@ -348,51 +345,54 @@ let ecdsa_signature_nist_compliant m privKey k result =
 
 val ecdsa_signature_core: mLen: size_t -> m: lbuffer uint8 mLen {uint_v mLen < pow2 61} ->  
   privKeyAsFelem: felem  -> 
-  kAsFelem: felem -> 
+  k: lbuffer uint8 (size 32) -> 
   r: felem -> 
   s: felem -> 
   Stack bool  
-  (requires fun h -> live h m /\ live h privKeyAsFelem /\ live h kAsFelem /\ live h r /\ live h s /\ 
-    LowStar.Monotonic.Buffer.all_disjoint [loc privKeyAsFelem |+| loc kAsFelem |+| loc r |+| loc s] /\
-    disjoint privKeyAsFelem r /\ disjoint kAsFelem r /\ disjoint r s /\
+  (requires fun h -> live h m /\ live h privKeyAsFelem /\ live h k /\ live h r /\ live h s /\ 
+    disjoint privKeyAsFelem r /\ disjoint k r /\ disjoint r s /\
     as_nat h privKeyAsFelem < prime_p256_order /\
-    as_nat h kAsFelem < prime_p256_order
+    Lib.ByteSequence.nat_from_bytes_le (as_seq h k) < prime_p256_order
   )
-  (ensures fun h0 flag h1 -> 
+  (ensures fun h0 flag h1 -> modifies (loc r |+| loc s) h0 h1 /\
     (
-      let hashOfMessage = Spec.Hash.hash Spec.Hash.Definitions.SHA2_256 (as_seq h0 m) in 
-      let changedEndianHash = Hacl.Spec.ECDSA.changeEndian (Lib.ByteSequence.uints_from_bytes_be hashOfMessage) in 
-      let z = felem_seq_as_nat changedEndianHash % prime_p256_order in 
-
+      let hashM = Spec.Hash.hash Spec.Hash.Definitions.SHA2_256 (as_seq h0 m) in 
+      let hashChanged = Hacl.Spec.ECDSA.changeEndian (Lib.ByteSequence.uints_from_bytes_be hashM) in
+      let z = (Lib.ByteSequence.nat_from_intseq_le hashChanged) % prime_p256_order in 
+      
       let basePoint = (0x6B17D1F2E12C4247F8BCE6E563A440F277037D812DEB33A0F4A13945D898C296, 0x4FE342E2FE1A7F9B8EE7EB4A7C0F9E162BCE33576B315ECECBB6406837BF51F5, 1) in
-      let k = Lib.ByteSequence.uints_to_bytes_le (as_seq h0 kAsFelem) in 
-      let (rxN, ryN, rzN), _ = montgomery_ladder_spec k ((0,0,0), basePoint) in 
+      let (rxN, ryN, rzN), _ = montgomery_ladder_spec (as_seq h0 k) ((0,0,0), basePoint) in 
       let (xN, _, _) = _norm (rxN, ryN, rzN) in 
+      
+      let kFelem = Lib.ByteSequence.nat_from_bytes_le (as_seq h0 k) in 
       as_nat h1 r == xN % prime_p256_order /\
       (
-	if as_nat h1 r = 0 then flag = false else 
-	  as_nat h1 s == (z + (as_nat h1 r) * as_nat h0 privKeyAsFelem) * pow (as_nat h0 kAsFelem) (prime_p256_order - 2) % prime_p256_order /\
-	  (
-	    if (as_nat h1 s = 0) then 
-	      flag = false else flag = true
-	  )
+	if as_nat h1 r = 0 then flag = false else
+	  as_nat h1 s == (z + (as_nat h1 r) * as_nat h0 privKeyAsFelem) * pow kFelem (prime_p256_order - 2) % prime_p256_order /\
+	(
+	  if (as_nat h1 s = 0) then flag = false else flag = true
+	)
       )
-    )
+    )    
 )
 
-let ecdsa_signature_core mLen m privKeyAsFelem kAsFelem r s = 
+
+let ecdsa_signature_core mLen m privKeyAsFelem k r s = 
   push_frame();
     let h0 = ST.get() in 
       let hashAsFelem = create (size 4) (u64 0) in     
       let tempBuffer = create (size 100) (u64 0) in 
-      let k8 = create (size 32) (u8 0) in 
-      toUint8 kAsFelem k8;
-      ecdsa_signature_step12 mLen m hashAsFelem;
+      let kAsFelem = create (size 4) (u64 0) in 
+    toUint64 k kAsFelem;  
+    ecdsa_signature_step12 mLen m hashAsFelem;
+
   let h1 = ST.get() in 
-    let step5Flag = ecdsa_signature_step45 k8 tempBuffer r in 
+      lemma_core_0 kAsFelem h1;
+      uints_from_bytes_le_nat_lemma #U64 #_ #4 (as_seq h0 k);
+    let step5Flag = ecdsa_signature_step45 k tempBuffer r in 
       if not step5Flag then begin
 	ecdsa_signature_step6 kAsFelem hashAsFelem r privKeyAsFelem s;
-	pop_frame();
+	pop_frame(); 
 	let step6Flag = isZero_bool s in 
 	not step6Flag
       end
@@ -403,31 +403,77 @@ let ecdsa_signature_core mLen m privKeyAsFelem kAsFelem r s =
       end   
 
 
-
-val ecdsa_signature:  mLen: size_t -> m: lbuffer uint8 mLen {uint_v mLen < pow2 61} -> privKey: lbuffer uint8 (size 32) -> 
+val ecdsa_signature:  mLen: size_t -> m: lbuffer uint8 mLen {uint_v mLen < pow2 61} ->
+  privKey: lbuffer uint8 (size 32) -> 
   k: lbuffer uint8 (size 32) -> 
   result: lbuffer uint8 (size 64) -> Stack bool
-  (requires fun h -> live h privKey /\ live h k /\ live h result /\ live h m)
-  (ensures fun h0 _ h1 -> True)
+  (requires fun h -> live h privKey /\ live h k /\ live h result /\ live h m /\
+    LowStar.Monotonic.Buffer.all_disjoint [loc m; loc privKey; loc k; loc result] /\
+    
+    Lib.ByteSequence.nat_from_bytes_le (as_seq h privKey) < prime_p256_order /\
+    Lib.ByteSequence.nat_from_bytes_le (as_seq h m) < prime_p256_order /\
+    Lib.ByteSequence.nat_from_bytes_le (as_seq h k) < prime_p256_order
+  )
+  (ensures fun h0 flag h1 -> modifies (loc result) h0 h1 /\
+     (
+       
+      let resultR = gsub result (size 0) (size 32) in 
+      let resultS = gsub result (size 32) (size 32) in 
+      
+
+      let hashM = Spec.Hash.hash Spec.Hash.Definitions.SHA2_256 (as_seq h0 m) in 
+      let hashChanged = Hacl.Spec.ECDSA.changeEndian (Lib.ByteSequence.uints_from_bytes_be hashM) in
+      let z = (Lib.ByteSequence.nat_from_intseq_le hashChanged) % prime_p256_order in 
+
+      let privateKey = Lib.ByteSequence.nat_from_bytes_le (as_seq h0 privKey) in 
+
+      let basePoint = (0x6B17D1F2E12C4247F8BCE6E563A440F277037D812DEB33A0F4A13945D898C296, 0x4FE342E2FE1A7F9B8EE7EB4A7C0F9E162BCE33576B315ECECBB6406837BF51F5, 1) in
+      let (rxN, ryN, rzN), _ = montgomery_ladder_spec (as_seq h0 k) ((0,0,0), basePoint) in 
+      let (xN, _, _) = _norm (rxN, ryN, rzN) in 
+      
+      let kFelem = Lib.ByteSequence.nat_from_bytes_le (as_seq h0 k) in 
+     
+      let resultR = nat_from_bytes_le (as_seq h1 resultR) in 
+      let resultS = nat_from_bytes_le (as_seq h1 resultS) in 
+
+      resultR == xN % prime_p256_order /\
+      (
+	if resultR = 0 then flag = false else
+	  resultS == (z + resultR * privateKey) * pow kFelem (prime_p256_order - 2) % prime_p256_order /\
+	(
+	  if (resultS = 0) then flag = false else flag = true
+	)
+      )
+    )    
+)
 
 
 let ecdsa_signature mLen m privKey k result = 
   push_frame();
-    let kAsFelem = create (size 4) (u64 0) in 
-    let privKeyAsFelem = create (size 4) (u64 0) in 
-    let r = create (size 4) (u64 0) in 
-    let s = create (size 4) (u64 0) in 
+    let h0 = ST.get() in 
+      let privKeyAsFelem = create (size 4) (u64 0) in 
+      let r = create (size 4) (u64 0) in 
+      let s = create (size 4) (u64 0) in 
 
-    let resultR = sub result (size 0) (size 32) in 
-    let resultS = sub result (size 32) (size 32) in 
-      toUint64 privKey privKeyAsFelem;
-	reduction_prime_2prime_order privKeyAsFelem privKeyAsFelem;
-      toUint64 k kAsFelem;
-	reduction_prime_2prime_order kAsFelem kAsFelem;
+      let resultR = sub result (size 0) (size 32) in 
+      let resultS = sub result (size 32) (size 32) in 
+	toUint64 privKey privKeyAsFelem;
 
-    let flag = ecdsa_signature_core mLen m privKeyAsFelem kAsFelem r s in 
+    let h1 = ST.get() in 
+      lemma_core_0 privKeyAsFelem h1;
+      Lib.ByteSequence.uints_from_bytes_le_nat_lemma #U64 #_ #4 (as_seq h1 privKey);
+      
+    let flag = ecdsa_signature_core mLen m privKeyAsFelem k r s in 
+      let h2 = ST.get() in 
+
       toUint8 r resultR;
       toUint8 s resultS;
+
+      lemma_core_1 r h2;
+      lemma_core_1 s h2;
+
+      pop_frame();
+
     flag  
 
     
